Working on progress.. A lot of typo found.

src/SSmtyP.v
@@ -48,7 +48,14 @@ Theorem rcd_field_ty_well_formed:
     inversion h'; subst; eauto.
 Qed.
 
-
+Theorem rcd_field_ty_not_TNone:
+    forall rcd h h' i T,
+        rcd_field_ty rcd h h' i = Some T ->
+        rcd <> TNone.
+    intros rcd h. induction h; intros; intro; subst; eauto.
+    inversion H; subst; eauto.
+    inversion H0.
+Qed.
 
 
 
@@ -174,6 +181,8 @@ Inductive value : tm -> Prop :=
                 value (tright T wft t)
     | vfield : forall T ort wft id,
                 value (tfield T ort wft id).
+
+Hint Constructors value.
 
 (* subst (i:id) (rep: tm) (org: tm) : tm *)
 Definition subst : id -> tm -> tm -> tm.
@@ -433,6 +442,16 @@ Inductive step : tm -> tm -> Prop :=
             value lb ->
             step rb rb' ->
             step (tcase crit lb rb) (tcase crit lb rb')
+    | stcase3 :
+        forall lt LT RT w0 w1 i0 i1 body0 body1,
+            value lt ->
+            step (tcase (tleft lt RT w1) (tfun i0 LT w0 body0) (tfun i1 RT w1 body1))
+                    (tapp (tfun i0 LT w0 body0) lt)
+    | stcase4 :
+        forall rt LT RT w0 w1 i0 i1 body0 body1,
+            value rt ->
+            step (tcase (tright LT w0 rt) (tfun i0 LT w0 body0) (tfun i1 RT w1 body1))
+                    (tapp (tfun i1 RT w1 body1) rt)
     | stfield0 :
         forall T orcd w i j head tail,
             value (trcons j head tail) ->
@@ -534,12 +553,25 @@ Theorem step_deterministic:
         | h0 : step (tfield ?T ?ort ?wft ?i) _ |- _ =>
             poses' (vfield T ort wft i)
     end;
-    try tac_value_no_step; 
+    
     try (match goal with
         | h0 : ?x <> ?x |- _ => destruct (h0 eq_refl)
         end
     );
-    fail).
+    try 
+    match goal with
+        | h0 : step (tleft ?lt ?RT ?w1) _, h1: value ?lt |- _ =>
+            poses' (vleft lt RT w1 h1)
+    end;
+    try 
+    match goal with
+        | h0 : step (tright ?LT ?w0 ?rt) _, h1: value ?rt |- _ =>
+            poses' (vright LT w0 rt h1)
+    end;
+    try tac_value_no_step; 
+    fail
+    ).
+
     (* tlet, wf_ty difference *)
     erewrite (wf_ty_indistinct T w w1); eauto.
     (* tfix, wf_ty difference *)
@@ -550,9 +582,16 @@ Theorem step_deterministic:
     erewrite (wf_ty_indistinct w R R1); eauto.
     (* tright, wf_ty difference *)
     erewrite (wf_ty_indistinct w L L1); eauto.
-    (* tfield , wf_ty orcd difference*)
-    erewrite (wf_ty_indistinct T w w1);
+
+
+    (* tcase , wf_ty orcd difference*)
+    erewrite (wf_ty_indistinct LT w0 w5); eauto.
+
+    (* tcase , wf_ty orcd difference*)
+    erewrite (wf_ty_indistinct RT w1 w5); eauto.
+    (*tfield, wf_ty orcd difference*)
     erewrite (orcd_indistinct T orcd orcd1); eauto.
+    erewrite (wf_ty_indistinct T w w1); eauto.
 Qed.
 
 Ltac glize_aux x L :=
@@ -591,6 +630,21 @@ Lemma ext_type_tchr:
         end
     ).
 Qed.
+
+Lemma ext_type_tfun:
+    forall t,
+        value t ->
+        forall iT oT,
+        has_type empty t (TFun iT oT) ->
+        (exists i T w body, t = tfun i T w body) \/ (exists T o w i, t = tfield T o w i).
+        intros t h0;
+    induction h0; intros; subst; eauto; try discriminate;
+    try (match goal with
+            | H0 : has_type _ _ _ |- _ => inversion H0; subst; eauto
+        end
+    ); [left | right]; eexists; eauto.
+Qed.
+
 
 Lemma ext_type_tbool:
     forall t,
@@ -635,6 +689,40 @@ Lemma ext_type_tnone:
     ).
 Qed.
 
+Lemma ext_type_trcd:
+    forall t,
+        value t ->
+        forall T,
+        has_type empty t T ->
+        T <> TNone ->
+        only_rcd T ->
+        wf_ty T ->
+        exists i th tt, t = trcons i th tt.
+    intros t h0;
+    induction h0; intros; subst; eauto; try discriminate;
+    try (match goal with
+            | H0 : has_type _ _ _ |- _ => inversion H0; subst; eauto
+        end;
+        match goal with
+            | h: only_rcd (TFun _ _) |- _ => inversion h; subst; eauto
+            | H0 : only_rcd _ |- _ => inversion H0; subst; eauto
+        end;
+        try discriminate
+    ).
+    (* Case: TNone*)
+    destruct (H0 eq_refl).
+Qed.
+
+
+Ltac destructALL :=
+    repeat (
+        match goal with
+        | h0: _ \/ _ |- _ => destruct h0
+        | h0: _ /\ _ |- _ => destruct h0
+        | h0: exists _, _ |- _ => destruct h0
+        end
+    ).
+
 
 Theorem progress:
     forall t T,
@@ -669,20 +757,14 @@ Theorem progress:
     end;
     left; eauto; fail
     );
+    repeat (match goal with
+    | h0: ?X = ?X -> _ |- _ => poses' (h0 eq_refl); clear h0
+    end);
     try (
     assert(ttrue <> tfalse); try (intro; discriminate);eauto;
     assert(tfalse <> ttrue); try (intro; discriminate);eauto;
     right; 
-    repeat (match goal with
-            | h0: ?X = ?X -> _ |- _ => poses' (h0 eq_refl); clear h0
-            end);
-    repeat (match goal with
-            | h0 : _ \/ _ |- _ => destruct h0
-            end);
-    repeat (match goal with
-            | h0 : exists _ : _, _ |- _ => destruct h0
-            end);
-        try 
+    destructALL;
             (repeat (match goal with
                 | h0 : value ?X, h1: has_type empty ?X TNat |- _=> 
                     destruct (ext_type_tnat _ h0 h1); subst; eauto; generalize dependent h0; generalize dependent h1
@@ -694,8 +776,38 @@ Theorem progress:
                     destruct (ext_type_tsum _ h0 h1); subst; eauto; generalize dependent h0; generalize dependent h1
                 | h0 : value ?X, h1: has_type empty ?X TNone |- _=> 
                     destruct (ext_type_tnone _ h0 h1); subst; eauto; generalize dependent h0; generalize dependent h1
+                | h0 : value ?X, h1: has_type empty ?X (TFun _ _) |- _=> 
+                    destruct (ext_type_tfun _ h0 _ _ h1); destructALL; subst; eauto; generalize dependent h0; generalize dependent h1
+                | h0 : value ?X, h1: has_type empty ?X (TSum _ _) |- _=> 
+                    destruct (ext_type_tsum _ h0 _ _ h1); destructALL; subst; eauto; generalize dependent h0; generalize dependent h1
             end));intros;
-    eexists; eauto). eapply eauto.
+    eexists; eauto; fail
+    ).
+
+    (* case: trcons *)
+    destructALL;
+    match goal with
+    | h0 : value ?t0, h1: value ?t1 |- _ => left; eauto
+    | |- _ => right; eexists; eauto
+    end.
+
+    (* case: tapp*)
+    right; 
+    destructALL;
+            (repeat (match goal with
+                 | h0 : value ?X, h1: has_type empty ?X (TFun _ _) |- _=> 
+                    destruct (ext_type_tfun _ h0 _ _ h1); destructALL; subst; eauto; generalize dependent h0; generalize dependent h1
+                  end));intros;
+    eexists; eauto.
+        (* case: tapp: tfield*)
+    inversion h1_1; subst; eauto. 
+    poses' (rcd_field_ty_not_TNone _ _ _ _ _ H3).
+    poses' (ext_type_trcd _ H0 _ h1_2 H1 x0 x1); destructALL; subst; eauto.
+    inversion h1_2; subst; eauto. destruct (eq_id_dec x x2); subst; eauto; try discriminate. eapply stfield1.
+
+    inversion h1_1; subst; eauto. 
+    destruct (ext_type_tfun _ H1 h1_1); destructALL; subst; eauto.
+    eapply eauto.
 
 Theorem preservation:
     forall t t' T,
